theories/stablesort.v
@@ -1,4 +1,3 @@
-From stablesort Require Import mathcomp_ext.
 From mathcomp Require Import ssreflect ssrfun ssrbool eqtype ssrnat seq path.
 From stablesort Require Import param.
 
@@ -6,7 +5,28 @@ Set Implicit Arguments.
 Unset Strict Implicit.
 Unset Printing Implicit Defensive.
 
-Local Notation count_merge := mathcomp_ext.count_merge.
+Local Definition condrev (T : Type) (r : bool) (xs : seq T) : seq T :=
+  if r then rev xs else xs.
+
+Local Lemma condrev_nilp (T : Type) (r : bool) (xs : seq T) :
+  nilp (condrev r xs) = nilp xs.
+Proof. by case: r; rewrite /= ?rev_nilp. Qed.
+
+Local Lemma relpre_trans {T' T} {leT : rel T} {f : T' -> T} :
+  transitive leT -> transitive (relpre f leT).
+Proof. by move=> + y x z; apply. Qed.
+
+Local Lemma allrel_rev2 {T S} (r : T -> S -> bool) (s1 : seq T) (s2 : seq S) :
+  allrel r (rev s1) (rev s2) = allrel r s1 s2.
+Proof. by rewrite [LHS]all_rev [LHS]allrelC [RHS]allrelC [LHS]all_rev. Qed.
+
+Local Lemma count_merge (T : Type) (leT : rel T) (p : pred T) (s1 s2 : seq T) :
+  count p (merge leT s1 s2) = count p (s1 ++ s2).
+Proof.
+rewrite count_cat; elim: s1 s2 => // x s1 IH1.
+elim=> //= [|y s2 IH2]; first by rewrite addn0.
+by case: (leT x); rewrite /= ?IH1 ?IH2 ?[p y + _]addnCA addnA.
+Qed.
 
 (******************************************************************************)
 (* The abstract interface for stable (merge)sort algorithms                   *)
@@ -943,6 +963,33 @@ Canonical CBVAcc.sortN_stable.
 (******************************************************************************)
 
 Section StableSortTheory.
+
+Let lexord (T : Type) (leT leT' : rel T) :=
+  [rel x y | leT x y && (leT y x ==> leT' x y)].
+
+Local Lemma lexord_total (T : Type) (leT leT' : rel T) :
+  total leT -> total leT' -> total (lexord leT leT').
+Proof.
+move=> leT_total leT'_total x y /=.
+by move: (leT_total x y) (leT'_total x y) => /orP[->|->] /orP[->|->];
+  rewrite /= ?implybE ?orbT ?andbT //= (orbAC, orbA) (orNb, orbN).
+Qed.
+
+Local Lemma lexord_trans (T : Type) (leT leT' : rel T) :
+  transitive leT -> transitive leT' -> transitive (lexord leT leT').
+Proof.
+move=> leT_tr leT'_tr y x z /= /andP[lexy leyx] /andP[leyz lezy].
+rewrite (leT_tr _ _ _ lexy leyz); apply/implyP => lezx; move: leyx lezy.
+by rewrite (leT_tr _ _ _ leyz lezx) (leT_tr _ _ _ lezx lexy); exact: leT'_tr.
+Qed.
+
+Local Lemma lexord_irr (T : Type) (leT leT' : rel T) :
+  irreflexive leT' -> irreflexive (lexord leT leT').
+Proof. by move=> irr x /=; rewrite irr implybF andbN. Qed.
+
+Local Lemma lexordA (T : Type) (leT leT' leT'' : rel T) :
+  lexord leT (lexord leT' leT'') =2 lexord (lexord leT leT') leT''.
+Proof. by move=> x y /=; case: (leT x y) (leT y x) => [] []. Qed.
 
 Section StableSortTheory_Part1.
 
